%%%%%%%%%%%%%%%%%%%%%%%%%%%%%%%%%%%%%%%%%%%%%%%%%%%%%%%%%%%%%%%%%%%%%%%%%%%%%%%%
% reconstruction.tex:
%%%%%%%%%%%%%%%%%%%%%%%%%%%%%%%%%%%%%%%%%%%%%%%%%%%%%%%%%%%%%%%%%%%%%%%%%%%%%%%%
\chapter{Multiple Choice}
\label{Multiple Choice}
%%%%%%%%%%%%%%%%%%%%%%%%%%%%%%%%%%%%%%%%%%%%%%%%%%%%%%%%%%%%%%%%%%%%%%%%%%%%%%%%
problem 1: c

problem 2: c

problem 3: d

$v_{ag}$ = speed of air relative to ground = $65 \frac{miles}{hour}$ constant speed on both trips
$v_{pg}$ = speed of plane relative to ground = constant speed on both trips
D = distance between A and B = $2300 miles$
$T_{A \rightarrow B} = \frac{D}{v_{pg} - v_{ag}}$
$T_{B \rightarrow A} = \frac{D}{v_{pg} + v_{ag}}$
                                                                 
$T_{A \rightarrow B} - T_{B \rightarrow A}$ = $65$ minutes = $\frac{65}{60}$ hours
$T_{A \rightarrow B} - T_{B \rightarrow A}$ = $\frac{D}{v_{pg} - v_{ag}} - \frac{D}{v_{pg} + v_{ag}}$
                                                                   
rearranging the right side of the equation to make one fraction yields
$T_{A \rightarrow B} - T_{B \rightarrow A}$ = D$\frac{2v_{ag}}{v_{pg}^{2} - v_{ag}^{2}}$

                                                                 
solving for the speed of the plane relative to the ground $v_{pg}$ gives
$v_{pg}^{2}$ = $v_{ag}^{2} + \frac{2Dv_{ag}}{T_{A \rightarrow B} - T_{B \rightarrow A}}$
$v_{pg} = 529.4 \frac{miles}{hour}$

problem 4: a
                                                     
given the acceleration $a_{e}$ and applied force $F_{app}$ on earth, the mass M can be calculated
$M = \frac{F_{app}}{a_{e}} = \frac{90 N}{1.9 \frac{m}{s^{2}}} = 47.4$ kg
                                              
weight on the moon $W_{moon}$ = $Ma_{moon}$ = $(47.4 kg)(1.62 \frac{m}{s^{2}} )$ = $76.7 N$

problem 5: b

use momentum conservation to determine final velocity of the heavier mass $m_{B}$
$m_{A} = 2.0$ kg  initial speed $v_{A0} = 20.0 \frac{m}{s}$ to the east
$m_{B} = 3.0$ kg  initial speed $v_{B0} = 20.0 \frac{m}{s}$ to the west
$v_{Af} = 5.0 \frac{m}{s}$ to the west

$m_{B}v_{B0}$ - $m_{A}v_{A0}$ = $m_{A}v_{Af}$ + $m_{B}v_{Bf}$

solving for $v_{Bf}$ yields
$v_{Bf} = \frac{m_{B}v_{B0} - m_{A}v_{A0} - m_{A}v_{Af}}{m_{B}}$
$v_{Bf} = \frac{10}{3} \frac{m}{s} = 3.3 \frac{m}{s}$ to the west
                                                 
the kinetic energy lost is equal to the difference between the initial kinetic
energy $KE_{0}$ and final kinetic energy $KE_{f}$
$KE_{0} - KE_{f}$ = (1/2)($m_{A}v_{A0}^{2} + m_{B}v_{B0}^{2} - m_{A}v_{Af}^{2} - m_{B}v_{Bf}^{2}$)
$KE_{0} - KE_{f} = 958$ Joules
%%%%%%%%%%%%%%%%%%%%%%%%%%%%%%%%%%%%%%%%%%%%%%%%%%%%%%%%%%%%%%%%%%%%%%%%%%%%%%%%
